src/program_proof/append_log_proof.v
@@ -893,96 +893,44 @@ Qed.
 
 End heap.
 
+Section crash.
+Context `{!heapG Σ}.
+
 Instance is_hdr_durable sz disk_sz:
-  IntoCrash (λ _ _, is_hdr sz disk_sz) (λ _ _, is_hdr sz disk_sz).
+  IntoCrash (is_hdr sz disk_sz) (λ _, is_hdr sz disk_sz).
 Proof. apply _. Qed.
 
 Instance is_log'_durable sz disk_sz vs:
-  IntoCrash (λ _ _, is_log' sz disk_sz vs) (λ _ _, is_log' sz disk_sz vs).
+  IntoCrash (is_log' sz disk_sz vs) (λ _, is_log' sz disk_sz vs).
 Proof. apply _. Qed.
 
 Instance crashed_log_durable bs:
-  IntoCrash (λ _ _, crashed_log bs) (λ _ _, crashed_log bs).
+  IntoCrash (crashed_log bs) (λ _, crashed_log bs).
 Proof. apply _. Qed.
 
 Instance uninit_log_durable sz:
-  IntoCrash (λ _ _, uninit_log sz) (λ _ _, uninit_log sz).
+  IntoCrash (uninit_log sz) (λ _, uninit_log sz).
 Proof. apply _. Qed.
 
 Instance unopened_log_durable sz:
-  IntoCrash (λ _ _, unopened_log sz) (λ _ _, unopened_log sz).
+  IntoCrash (unopened_log sz) (λ _, unopened_log sz).
 Proof. apply _. Qed.
 
-(*
-From iris.proofmode Require Import base intro_patterns spec_patterns
-                                   sel_patterns coq_tactics reduction.
-
-From Perennial.Helpers Require Import NamedProps.
-
-Ltac apply_into_crash id A :=
-  let Hpose := fresh "Hpose" in
-  pose proof (_ : IntoCrash (λ _ _, A) _) as Hpose.
-(*  iEval (rewrite Hpose) in id; clear Hpose *)
-
-Ltac crash_env Γ :=
-  match Γ with
-    | environments.Enil => idtac
-    | environments.Esnoc ?Γ' ?id ?A => first [ apply_into_crash id A || iClear id ] ; crash_env Γ'
-  end.
-
-Ltac iCrash :=
-  match goal with
-  | [ |- environments.envs_entails ?Γ _] =>
-    let H := iFresh in
-    let spatial := pm_eval (environments.env_spatial Γ) in
-    let intuit := pm_eval (environments.env_intuitionistic Γ) in
-    crash_env spatial; crash_env intuit
-    (*
-    iApply (modus_ponens with "[-]"); [ iNamedAccu | ];
-    rewrite ?post_crash_named ?post_crash_sep
-     *)
-  end.
-
 Instance ptsto_log_into_crash l vs:
-  IntoCrash (λ _ _, ptsto_log l vs) (λ _ _, crashed_log vs).
+  IntoCrash (ptsto_log l vs) (λ _, crashed_log vs).
 Proof.
-  iIntros (??) "HP". iDestruct "HP" as (??) "(H1&H2)". 
-  Check into_crash.
-  Print Instances IntoCrash.
-  Check @into_crash.
-  apply_into_crash "H2" (is_log' H H0 vs).
-  iCrash.
-  pose proof (_ : IntoCrash (λ _ _, is_log' H H0 vs) _) as Hfoo.
-  rewrite Hfoo.
-  rewrite (@into_crash _ _ _ _ _ (is_log'_durable _ _ _)). iCrash.
-  iIntros 
- apply _. Qed.
+  rewrite /IntoCrash.
+  iIntros "HP". iDestruct "HP" as (??) "(H1&H2)".
+  (* log_fields gets cleared because it's not durable, is_log' sticks around *)
+  iCrash. iExists _, _. eauto.
+Qed.
 
-(*
-From iris.proofmode Require Import tactics monpred.
-Instance heapG_index_heapG {Σ} (hGi: heapG_index (Σ := Σ)) : heapG Σ.
-Proof. move: hGi. rewrite /heapG_index//=. Defined.
-
-Existing Instance FromModal_post_crash.
-
-Definition fun2monpred {Σ} (P : heapG Σ → iProp Σ) : monPred (heapG_index (Σ := Σ)) (iPropI Σ) :=
-  {| monPred_at := (λ hG, P (heapG_index_heapG hG)) |}.
-
-Notation "'<>' P" := (fun2monpred (λ H, P)) (at level 100) : bi_scope.
-
-Instance IntoCrash_IntoCrash' {Σ} (P: ∀ Σ, heapG Σ → iProp Σ) Q:
-  IntoCrash (P) Q →
-  IntoCrash' (fun2monpred (P Σ))%I (fund2monpred(Q Σ))%I.
-
-Instance is_log'_durable' {Σ} sz disk_sz vs:
-  IntoCrash' (Σ := Σ) (<> is_log' sz disk_sz vs)%I (<> is_log' sz disk_sz vs)%I.
-
-Lemma ptsto_log_post_crash {Σ: gFunctors} (l:loc) (vs:list Block) disk_sz sz:
-  (<> log_fields l sz disk_sz) -∗ (<> is_log' sz disk_sz vs) -∗ post_crash' (Σ := Σ) (<> crashed_log vs).
+Lemma ptsto_log_into_crash_test l vs:
+  ptsto_log l vs -∗ post_crash (λ hG, crashed_log vs).
 Proof.
-  iIntros "H1 H2".
-  iModIntro. iStopProof. iStartProof (iPropI Σ). iIntros (?) => //=.
-Abort.
+  iIntros "HP".
+  (* ptsto_log gets transformed into crashed_log when we go under the modality *)
+  iCrash. eauto.
+Qed.
 
-*)
-*)
+End crash.
